compose/SimMemId.v
@@ -47,10 +47,11 @@ Next Obligation.
   eexists (mkrelation _ _).
   esplits; ss; eauto.
   inv WF. ss.
-  inv WF0. ss. clear_tac.
-  assert(PUBS0: forall id, <<EQ: sk_src.(prog_defmap) ! id = sk_tgt.(prog_defmap) ! id>>).
-  { i. eapply PUBS. eauto. }
-  clear PUBS.
+  clear_tac.
+  assert(NOCOVER0: forall id, <<EQ: sk_src.(prog_defmap) ! id = sk_tgt.(prog_defmap) ! id>>).
+  { i. eapply NOCOVER. eauto. }
+  clear NOCOVER.
+  clear_tac.
   econs; eauto.
   - admit "This should hold; Maybe ""Genv.init_mem_match"" and ""Genv.init_mem_genv_next"" might help".
   - admit "This should hold;".
