compose/SimSymbKept.v
@@ -1,0 +1,19 @@
+Require Import Events.
+Require Import Values.
+Require Import AST.
+Require Import Asmregs.
+Require Import Memory.
+Require Import Globalenvs.
+Require Import Smallstep.
+Require Import CoqlibC.
+Require Import Skeleton.
+Require Import Integers.
+Require Import ASTC.
+Require Import LinkingC.
+Require Import SimSymb.
+Require Import MapsC.
+
+
+Set Implicit Arguments.
+
+
