lib/CoqlibC.v
@@ -13,6 +13,7 @@ Require Export Basics.
 Require Import Relations.
 Require Import RelationClasses.
 Require Import Wellfounded.
+Require Export Classical_Prop.
 
 Set Implicit Arguments.
 
